%!TeX spellcheck = en-US,en-DE

\begin{frame}[t]{Calculating sum}
  \vspace{0.5cm}
  To continue we need to find
  \only<1,3,4,5>{
    \begin{equation*}
      \begin{gathered}
        F(\valk, \vecr) = \frac{1}{\mathcal{V}} \sum_{\veck} e^{- i \textbf{k}\vecr}
        \bra{g} \hat c^{\dagger}_{\textbf{k}\sigma} \hat c_{\textbf{k}\sigma} \ket{g}
      \end{gathered}
    \end{equation*}
  }
  \only<2>{
    \begin{equation*}
      \begin{gathered}
        F(\valk, \vecr) = \frac{1}{\mathcal{V}} \sum_{\veck} e^{- i \textbf{k}\vecr}\:
        \textcolor{red}{
        \bra{g} \hat c^{\dagger}_{\textbf{k}\sigma} \hat c_{\textbf{k}\sigma} \ket{g}
        }
      \end{gathered}
    \end{equation*}
  }
  \only<3>{
    \begin{block}{Number of particles operator}
      $$ \hat c^{\dagger}_{\textbf{k}\sigma} \hat c_{\textbf{k}\sigma} = \hat n_{\textbf{k}\sigma}$$
    \end{block}
    %\vspace{0.5cm}
    \begin{equation*}
      \bra{g} \hat c^{\dagger}_{\textbf{k}\sigma} \hat c_{\textbf{k}\sigma} \ket{g} =
      \bra{g} \hat n_{\textbf{k}\sigma} \ket{g} =
      \begin{cases}
        1 \quad \valk \leq \valk_F\\
        0 \quad \valk > \valk_F
      \end{cases}
    \end{equation*}
  }

  \only<4>{
    \vspace{0.5cm}
    Heaviside step function
    \begin{equation*}
      \bra{g} \hat c^{\dagger}_{\textbf{k}\sigma} \hat c_{\textbf{k}\sigma} \ket{g} =
      H(\valk_F - \abs{\veck})
    \end{equation*}
  }

  \only<5>{
    \vspace{0.5cm}
    Change to summation inside the Fermi sphere
    \begin{equation*}
      F(\valk, \vecr) = \frac{1}{\mathcal{V}} \sum_{\abs{\veck}\leq \valk_F} e^{- i \textbf{k}\vecr}
    \end{equation*}
  }

\end{frame}

\begin{frame}{From summation to integration}
  Multiply and divide by unit cell volume
  \begin{equation*}
    F(\valk, \vecr) = \frac{1}{\mathcal{V}} \sum_{\abs{\veck}\leq \valk_F} e^{- i \textbf{k}\vecr} =
    \frac{1}{\mathcal{V}} \frac{\mathcal{V}}{ 8 \pi^3} \sum_{\abs{\veck}\leq \valk_F} e^{- i \textbf{k}\vecr} d^3\valk
  \end{equation*}
  \vspace{0.5cm}
  In the limit $\mathcal{V} \to \infty$
  \begin{equation*}
    F(\valk, \vecr) = \frac{1}{8 \pi^3} \sum_{\abs{\veck}\leq \valk_F} e^{- i \textbf{k}\vecr} d^3\valk
    \to
    \frac{1}{8 \pi^3} \int_{\abs{\veck}\leq \valk_F} e^{- i \textbf{k}\vecr} d^3\valk
  \end{equation*}
\end{frame}

\begin{frame}[t]{Evaluation of the integral}
  \vspace{0.2cm}
  We will integrate in spherical coordinates
  \only<1>{
    \begin{equation*}
      F(\valk, \vecr) = \frac{1}{8 \pi^3} \int_{\abs{\veck}\leq \valk_F} e^{- i \textbf{k}\vecr} d^3\valk
    \end{equation*}
  }
  \only<2>{
  \begin{equation*}
    F(\valk, \vecr) =
    \frac{1}{8 \pi^3} \int_{\valk = 0}^{\valk_F} \int_{\theta = 0}^{\pi} \int_{\phi = 0}^{2 \pi}
    e^{- i \text{k}r\cos{\theta}}\text{k}^2\sin{\theta} \: d \phi d\theta d \text{k}
  \end{equation*}
  }
  \vfill
  \begin{figure}
    \includegraphics[height=4cm]{sphcoordel}
    %\caption{}
    \label{sphcoordel}
  \end{figure}
\end{frame}

\begin{frame}{Evaluation of the integral}
  Integration over $\phi$

  % \only<>{
  % \begin{equation*}
  %   F(\valk, \vecr) =
  %   \frac{1}{8 \pi^3} \int_{\valk = 0}^{\valk_F} \int_{\theta = 0}^{\pi} \int_{\phi = 0}^{2 \pi}
  %   e^{- i \text{k}r\cos{\theta}}\text{k}^2\sin{\theta} \: d \phi d\theta d \text{k}
  % \end{equation*}
  % }

  \only<1>{
  \begin{equation*}
    F(\valk, \vecr) =
    \frac{1}{8 \pi^3} \int_{\valk = 0}^{\valk_F} \int_{\theta = 0}^{\pi}
    \textcolor{red}{\int_{\phi = 0}^{2 \pi}}
    e^{- i \text{k}r\cos{\theta}}\text{k}^2\sin{\theta} \: \textcolor{red}{d \phi} d\theta d \text{k}
  \end{equation*}
  }

  \only<1>{
  \begin{equation*}
    F(\valk, \vecr) =
    \frac{1}{4 \pi^2} \int_{\valk = 0}^{\valk_F} \int_{\theta = 0}^{\pi}
    e^{- i \text{k}r\cos{\theta}}\text{k}^2\sin{\theta} \: d\theta d \text{k}
  \end{equation*}
  }

\end{frame}

\begin{frame}{Evaluation of the integral}
  Integration over $\theta$

  \only<1,2>{
  \begin{equation*}
    F(\valk, \vecr) =
    \frac{1}{4 \pi^2} \int_{\valk = 0}^{\valk_F} \textcolor{red}{\int_{\theta = 0}^{\pi}}
    e^{- i \text{k}r\textcolor{red}{\cos{\theta}}}\text{k}^2
    \textcolor{red}{\sin{\theta} \: d\theta} d \text{k}
  \end{equation*}
  }

  \only<1,2>{
  \begin{equation*}
    F(\valk, \vecr) =
    \frac{1}{4 \pi^2} \int_{\valk = 0}^{\valk_F} \textcolor{red}{\int_{\theta = 0}^{\pi}}
    e^{- i \text{k}r\textcolor{red}{\cos{\theta}}}\text{k}^2 \: \textcolor{red}{-d\cos{\theta}} d \text{k}
  \end{equation*}
  }

  \only<1>{
  \begin{equation*}
    F(\valk, \vecr) =
    \frac{1}{4 \pi^2} \int_{\valk = 0}^{\valk_F} \textcolor{red}{\int_{\eta = -1}^{1}}
    e^{i \text{k}r\textcolor{red}{\eta}}\text{k}^2 \: \textcolor{red}{d\eta} d \text{k}
  \end{equation*}
  }

  \only<2>{
  \begin{equation*}
    F(\valk, \vecr) =
    \frac{1}{4 \pi^2} \int_{\valk = 0}^{\valk_F}
    \frac{2}{\text{k}r}\sin{(\text{k}r)} \: \text{k}^2 \: d \text{k}
  \end{equation*}
  }

\end{frame}

\begin{frame}[t]{Evaluation of the integral}
  \vspace{0.3cm}
  Integration over k

  \begin{equation*}
    F(\valk, \vecr) =
    \frac{1}{4 \pi^2} \int_{\valk = 0}^{\valk_F}
    \frac{2}{\text{k}r}\sin{(\text{k}r)} \: \text{k}^2 \: d \text{k} =
    \frac{1}{2 \pi^2 r^3} \int_{\valk = 0}^{\valk_F}
    \sin{(\text{k}r)} \: \text{k} r \: d \text{k}r
  \end{equation*}

  \only<1>{
  \begin{equation*}
    F(\valk, \vecr) =
    \frac{1}{2 \pi^2 r^3} \left \{ \sin(\valk_F r) - \valk_F r \cos(\valk_F r) \right \}
  \end{equation*}
  }

  \only<2>{
  \begin{equation*}
    F(\valk, \vecr) =
    \frac{\valk_F^3}{2 \pi^2 r^3 \valk_F^3} \left \{ \sin(\valk_F r) - \valk_F r \cos(\valk_F r) \right \}
  \end{equation*}

  \begin{block}{Fermi wavenumber}
    $$ \valk_F^3 = \frac{3 \pi^2 N}{\V}$$
  \end{block}
  }
\end{frame}

\begin{frame}{Evaluation of the integral}
  \begin{equation*}
    \frac{1}{\mathcal{V}} \sum_{\veck} e^{- i \textbf{k}\vecr}
    \bra{g} \hat c^{\dagger}_{\textbf{k}\sigma} \hat c_{\textbf{k}\sigma} \ket{g} =
    \left ( \frac{N}{2\mathcal{V}} \right )
    \frac{3 \left \{ \sin(\valk_F r) - \valk_F r \cos(\valk_F r) \right \} }{(k_F r)^3}
  \end{equation*}

  \vspace{1cm}
  No divergence at zero: at $\valk_F r \to 0 \iff r \ll \lambda_F$
  \begin{equation*}
    3 \frac{\sin(k_F r) - k_F r \cos(k_F r)}{(k_F r)^3} \approx
    3 \frac{x - x^3/6 - x (1 - x^2/2)}{x^3} = 3 \frac{1}{3} = 1
  \end{equation*}
\end{frame}
